Core/Reduction/Congr.lean
@@ -1,4 +1,8 @@
+import LeanSubst
+import Core.Term
 import Core.Reduction.Definition
+
+open LeanSubst
 
 -- Ctor2 Congr1
 @[simp]
@@ -53,3 +57,35 @@ theorem TyBindVariant.congr_lamt : congr lamt = false := by simp [congr]
 
 @[simp]
 theorem TyBindVariant.congr_allc : congr allc = true := by simp [congr]
+
+theorem Red.spine_congr_step :
+  Red G t t' ->
+  Red G (t.apply sp) (t'.apply sp)
+:= by
+  intro h
+  induction sp generalizing t t'
+  case nil => simp [Term.apply]; exact h
+  case cons hd tl ih =>
+    cases hd
+    case type A =>
+      simp [Term.apply]
+      apply ih; apply Red.ctor1_congr h
+    case term a =>
+      simp [Term.apply]
+      apply ih; apply Red.ctor2_congr1 _ h
+      simp
+    case oterm a =>
+      simp [Term.apply]
+      apply ih; apply Red.ctor2_congr1 _ h
+      simp
+
+theorem Red.spine_congr :
+  Star (Red G) t t' ->
+  Star (Red G) (t.apply sp) (t'.apply sp)
+:= by
+  intro h
+  induction h
+  case _ => apply Star.refl
+  case _ y z h1 h2 ih =>
+    apply Star.step ih
+    apply spine_congr_step h2
