Core/Term.lean
@@ -3,3 +3,4 @@ import Core.Term.BEq
 import Core.Term.Substitution
 import Core.Term.Spine
 import Core.Term.Variant
+import Core.Term.Telescope
