Core/Term/Telescope.lean
@@ -1,0 +1,135 @@
+import LeanSubst
+import Core.Util
+import Core.Ty
+import Core.Term.Definition
+import Core.Term.Substitution
+import Core.Term.BEq
+
+open LeanSubst
+
+def Term.telescope : Term -> Telescope × Term
+| lam A t =>
+  let (tl, b) := t.telescope
+  (.ty A :: tl, b)
+| Λ[K] t =>
+  let (tl, b) := t.telescope
+  (.kind K :: tl, b)
+| t => ([], t)
+
+def Term.tele_intro : Term -> Telescope -> Term
+| t, [] => t
+| t, .cons (.ty A) tl => λ[A] (t.tele_intro tl)
+| t, .cons (.kind K) tl => Λ[K] (t.tele_intro tl)
+
+theorem Term.telescope_eq_law {t : Term} :
+  t.telescope = (tele, b) ->
+  b.tele_intro tele = t
+:= by
+  intro j
+  induction tele generalizing t b
+  case nil =>
+    simp [Term.tele_intro]
+    cases t <;> try simp [Term.telescope, *] at j
+    all_goals try rw [j]
+    case tbind v _ _ =>
+    cases v <;> simp [Term.telescope] at j
+    rw [j]
+  case cons hd tl ih =>
+    sorry
+    -- cases hd
+    -- case kind K =>
+    --   simp [Term.tele_intro]
+    --   cases t <;> try simp [Term.telescope] at j
+    --   case tbind v K2 t =>
+    --   cases v <;> simp [Term.telescope] at j
+    --   rcases j with ⟨⟨e1, e2⟩, e3⟩; subst e1 e2 e3
+    --   generalize zdef : t.telescope = z at *
+    --   rcases z with ⟨ztele, z⟩ <;> simp at *
+    --   apply ih zdef
+    -- case ty A =>
+    --   simp [Term.tele_intro]
+    --   cases t <;> try  simp [Term.telescope] at j
+    --   case tbind v _ _=> cases v <;> simp [Term.telescope] at j
+    --   case lam C t =>
+    --     rcases j with ⟨⟨e1, e2⟩, e3⟩; subst e1 e2 e3
+    --     generalize zdef : t.telescope = z at *
+    --     rcases z with ⟨ztele, z⟩ <;> simp at *
+    --     apply ih zdef
+
+def Term.telescope_lam_count : Telescope -> Nat
+| [] => 0
+| .cons (.ty _) tl => telescope_lam_count tl + 1
+| .cons (.kind _) tl => telescope_lam_count tl
+
+@[simp]
+def tele_lift : Telescope -> Subst Term -> Subst Term
+| [], σ => σ
+| .cons (.ty _) te, σ => Subst.lift (tele_lift te σ)
+| .cons (.kind _) te, σ => (tele_lift te σ) ◾ +1@Ty
+
+@[simp]
+def tele_lift_ren : Telescope -> Ren -> Ren
+| [], r => r
+| .cons (.ty _) te, r => Ren.lift (tele_lift_ren te r)
+| .cons (.kind _) te, r => tele_lift_ren te r
+
+@[simp]
+theorem tele_lift_re : tele_lift te (re i :: σ) = re i :: tele_lift te σ := by
+  sorry
+
+@[simp]
+theorem tele_lift_succ : tele_lift te +1 = +1 := by sorry
+
+@[simp]
+theorem tele_lift_compose {σ τ : Subst Term}
+  : tele_lift te (σ ∘ τ) = tele_lift te σ ∘ tele_lift te τ
+:= by
+  sorry
+
+@[simp]
+theorem tele_lift_hcompose {σ : Subst Term} {τ : Subst Ty}
+  : tele_lift te (σ ◾ τ) = tele_lift te σ ◾ τ
+:= by
+  sorry
+
+@[simp]
+theorem telescope_subst {b : Term} :
+  (b.tele_intro te)[σ] = b[tele_lift te σ].tele_intro te
+:= by
+  induction te generalizing b σ
+  case nil => simp [Term.tele_intro]
+  case cons hd te ih =>
+    cases hd
+    case kind K =>
+      simp [Term.tele_intro]
+      replace ih := @ih (σ ◾ +1@Ty) b
+      simp at ih; apply ih
+    case ty A =>
+      simp [Term.tele_intro]
+      replace ih := @ih σ.lift b
+      simp at ih; apply ih
+
+-- theorem telescope_subst_ty {b : Term} :
+--   (b.tele_intro te)[σ:Ty] = b[tele_lift_ty te σ:Ty].tele_intro te
+-- := by
+--   induction te generalizing b σ
+--   case nil => simp [Term.tele_intro]
+--   case cons hd tl ih =>
+--     cases hd
+--     case kind K =>
+--       sorry
+--     case ty A =>
+--       simp [Term.tele_intro]
+--       sorry
+
+@[simp]
+def tele_lift_ty : Telescope -> Subst Ty -> Subst Ty
+| [], σ => σ
+| .cons (.ty _) te, σ => tele_lift_ty te σ
+| .cons (.kind _) te, σ => Subst.lift (tele_lift_ty te σ)
+
+@[simp]
+def tele_lift_iterated : Telescope -> IteratedSubst -> IteratedSubst
+| _, .nil => .nil
+| te, .term σ it => .term (tele_lift te σ) (tele_lift_iterated te it)
+| te, .type σ it => .type (tele_lift_ty te σ) (tele_lift_iterated te it)
